prove functional correctness for modular exponentiation (with Montgomery arithmetic)

specs/experimental/Spec.RSA.Lemmas.fst
@@ -21,14 +21,14 @@ let rec lemma_pow x n m =
   | 0 -> ()
   | _ -> lemma_pow x (n-1) m; ass x (pow x (n-1)) (pow x m)
 
-val lemma_pow2_greater_1: x:nat{x > 1} -> Lemma
+val lemma_pow_greater_0: a:nat{a > 0} -> b:nat -> Lemma
 	(requires True)
-	(ensures (pow2 (x - 1) > 1))
-	[SMTPat (pow2 (x - 1))]
-let rec lemma_pow2_greater_1 x =
-	match x with
-	| 2 -> ()
-	| _ -> lemma_pow2_greater_1 (x - 1)
+	(ensures (pow a b > 0))
+	[SMTPat (pow a b)]
+let rec lemma_pow_greater_0 a b =
+	match b with
+	| 0 -> ()
+	| _ -> lemma_pow_greater_0 a (b - 1)
 
 val lemma_pow_0: b:nat{b > 0} -> Lemma (pow 0 b = 0)
 let rec lemma_pow_0 b =
@@ -45,38 +45,64 @@ let rec lemma_pow_1 b =
 #reset-options "--z3rlimit 30 --max_fuel 0"
 
 val lemma_pow_pow:
-	a:nat -> b:nat -> c:nat -> Lemma (pow a (b * c) = pow (pow a b) c)
+	a:nat -> b:nat -> c:nat -> Lemma
+    (pow a (b * c) = pow (pow a b) c)
 let lemma_pow_pow a b c = admit()
 
+val lemma_pow_mul:
+	a:nat -> b:nat -> c:nat -> Lemma
+    (pow (a * b) c = (pow a c) * (pow b c))
+let lemma_pow_mul a b c = admit()
+
+val lemma_pow_div:
+    a:nat -> b:nat -> d:nat{d > 0} -> Lemma
+    (pow (a / d) b == (pow a b) / pow d b)
+let lemma_pow_div a b d = admit()
+
 val lemma_pow_a2_b:
-	a:nat -> b:nat -> Lemma (pow (a * a) b = pow a (2 * b))
+	a:nat -> b:nat -> Lemma 
+    (pow (a * a) b = pow a (2 * b))
 let lemma_pow_a2_b a b = admit()
 
 val lemma_pow_mod:
-	a:nat -> b:nat -> n:pos -> Lemma ((pow a b) % n == (pow (a % n) b) % n)
+	a:nat -> b:nat -> n:pos -> Lemma 
+    ((pow a b) % n == (pow (a % n) b) % n)
 let lemma_pow_mod a b n = admit()
 
-val lemma_div_mod:
-	a:nat -> p:pos -> Lemma (a = p * (a / p) + a % p)
-let lemma_div_mod a p = ()
+val lemma_mod_mult_div_1:
+    a:nat -> d:nat{d > 0} -> n:nat{n > 0} -> Lemma
+    ((a / d) % n == ((a % n) / d) % n)
+let lemma_mod_mult_div_1 a d n = admit()
 
-val lemma_mult_3:
-	a:nat -> b:nat -> c:nat -> Lemma (a * b * c = c * a * b)
-let lemma_mult_3 a b c = ()
+val lemma_mod_mult_div:
+    a:nat -> b:nat -> d:nat{d > 0} -> n:nat{n > 0} -> Lemma
+    ((a * b / d) % n == ((a % n) * b / d) % n)
+let lemma_mod_mult_div a b d n = admit()
+
+val lemma_mult_div_mod:
+    a:nat -> b:nat -> d:nat{d > 0} -> n:nat{n > 0} -> Lemma
+    ((a * (b / d)) % n == (a * b / d) % n)
+let lemma_mult_div_mod a b d n = admit()
+
+val lemma_div_lt_ab: a:nat -> b:nat -> d:pos -> Lemma
+    (requires (a < b))
+    (ensures (a / d < b / d))
+let lemma_div_lt_ab a b d = admit()
 
 (* LEMMAS for exponent blinding *)
 val lemma_mod_pq:
 	a:nat -> b:nat -> p:nat{p > 1} -> q:nat{q > 1} -> Lemma
-	(requires (a % p = b /\ a % q = b))
-	(ensures (a % (p * q) = b))
+	(requires (a % p == b /\ a % q == b))
+	(ensures (a % (p * q) == b))
 let lemma_mod_pq a b p q = admit()
 
 // m ^ (p - 1) = 1 (mod p) where m is any integer and p is a prime number
 val fermat_little_theorem:
-	p:nat{p > 1} -> m:nat -> Lemma ((pow m (p - 1)) % p = 1)
+	p:nat{p > 1} -> m:nat -> Lemma 
+    ((pow m (p - 1)) % p == 1)
 let fermat_little_theorem p m = admit()
 
-#reset-options "--z3rlimit 100 --max_fuel 0"
+#reset-options "--z3rlimit 150 --max_fuel 0"
 
 val lemma_exp_blinding_1:
 	n:nat{n > 1} -> phi_n:nat -> p:elem n{p > 1} ->
@@ -89,6 +115,19 @@ let lemma_exp_blinding_1 n phi_n p q m =
 	fermat_little_theorem q m;
 	lemma_pow_1 (p - 1);
 	assert ((pow m phi_n) % q == 1)
+
+val lemma_exp_blinding_2:
+	n:nat{n > 1} -> phi_n:nat -> p:elem n{p > 1} ->
+	q:elem n{q > 1} -> m:elem n -> Lemma
+	(requires (phi_n == (p - 1) * (q - 1) /\ n = p * q))
+	(ensures ((pow m phi_n) % (p * q) == 1))
+let lemma_exp_blinding_2 n phi_n p q m =
+	lemma_exp_blinding_1 n phi_n p q m;
+	assert ((pow m phi_n) % q == 1);
+	lemma_exp_blinding_1 n phi_n q p m;
+	assert ((pow m phi_n) % p == 1);
+	lemma_mod_pq (pow m phi_n) 1 p q;
+	assert ((pow m phi_n) % (p * q) == 1)
 
 #reset-options "--z3rlimit 300 --max_fuel 0"
 
@@ -105,39 +144,16 @@ let lemma_exp_blinding n phi_n p q d m r =
 	assert (pow m (phi_n * r) == pow (pow m phi_n) r);
 	lemma_pow_mod (pow m phi_n) r n;
 	assert ((pow (pow m phi_n) r) % n == (pow ((pow m phi_n) % n) r) % n);
-
-	lemma_exp_blinding_1 n phi_n p q m;
-	assert ((pow m phi_n) % q == 1);
-	lemma_exp_blinding_1 n phi_n q p m;
-	assert ((pow m phi_n) % p == 1);
-	lemma_mod_pq (pow m phi_n) 1 p q;
-	assert ((pow m phi_n) % n = 1);
+    lemma_exp_blinding_2 n phi_n p q m;
+    assert ((pow m phi_n) % (p * q) == 1);
 
 	lemma_pow_1 r;
 	modulo_lemma 1 n;
 	assert ((pow 1 r) % n = 1);
 	assert ((pow m (r * phi_n)) % n = 1);
-	lemma_mod_mul_distr_l (pow m (r * phi_n)) (pow m d) n;
-	assert (res == (((pow m (r * phi_n)) % n) * pow m d) % n);
-    assert ((pow m (d + r * phi_n)) % n  == (pow m d) % n)
-
-(* LEMMAS for modular exponentiation *)
-val lemma_mod_exp:
-	n:nat{n > 1} -> a:nat -> a2:nat ->
-	b:nat -> b2:nat -> acc:elem n -> res:nat -> Lemma
-	(requires (a2 == (a * a) % n /\ b2 == b / 2 /\ res == (pow a2 b2 * acc) % n))
-	(ensures (res == (pow a (2 * b2) * acc) % n))
-
-let lemma_mod_exp n a a2 b b2 acc res =
-	let res = (pow a2 b2 * acc) % n in
-	lemma_mod_mul_distr_l (pow a2 b2) acc n;
-	assert (((pow a2 b2) * acc) % n == ((pow a2 b2) % n * acc) % n);
-	lemma_pow_mod (a * a) b2 n;
-	assert ((pow a2 b2) % n == (pow (a * a) b2) % n);
-	lemma_pow_a2_b a b2;
-	assert ((pow (a * a) b2) % n == (pow a (2 * b2)) % n);
-	assert (res == ((pow a (2 * b2)) % n * acc) % n);
-	lemma_mod_mul_distr_l (pow a (2 * b2)) acc n
+	lemma_mod_mul_distr_l (pow m (r * phi_n)) (pow m d) n
+	//assert (res == (((pow m (r * phi_n)) % n) * pow m d) % n);
+    //assert ((pow m (d + r * phi_n)) % n  == (pow m d) % n)
 
 (* LEMMAS for Karatsuba's multiplication *)
 val lemma_distributivity_mult: a:int -> b:int -> c:int -> d:int -> Lemma
@@ -160,11 +176,12 @@ let lemma_karatsuba_mult x a a0 a1 b b0 b1 =
 	let pow_x1 = pow2 (pow2 (x + 1)) in
 	assert (a * b == (a1 * pow_x + a0) * (b1 * pow_x + b0));
 	lemma_distributivity_mult (a1 * pow_x) a0 (b1 * pow_x) b0;
-	assert (a * b == a1 * b1 * pow_x * pow_x + (a0 * b1 + a1 * b0) * pow_x + a0 * b0);
+	//assert (a * b == a1 * b1 * pow_x * pow_x + (a0 * b1 + a1 * b0) * pow_x + a0 * b0);
 	pow2_plus (pow2 x) (pow2 x);
 	assert (pow2 (pow2 x) * pow2 (pow2 x) == pow2 (pow2 x + pow2 x));
 	pow2_double_sum x;
-	assert (pow2 x + pow2 x == pow2 (x + 1))
+	assert (pow2 x + pow2 x == pow2 (x + 1));
+    distributivity_add_left (a0 * b1) (a1 * b0) pow_x
 
 #reset-options "--z3rlimit 100 --initial_fuel 0 --max_fuel 0"
 
@@ -189,19 +206,152 @@ val abs: x:int -> Tot (y:int{ (x >= 0 ==> y = x) /\ (x < 0 ==> y = -x) })
 let abs x = if x >= 0 then x else -x
 
 (* LEMMAS for Montgomery's arithmetic *)
-#reset-options "--max_fuel 0"
-
-val lemma_div_lt_ab: a:nat -> b:nat -> d:pos -> Lemma
-    (requires (a < b))
-    (ensures (a / d < b / d))
-let lemma_div_lt_ab a b d = admit()
+#reset-options "--z3rlimit 150 --max_fuel 0"
 
 val lemma_mod_div_simplify: a:nat -> r:nat{r > 0} -> n:nat{n > 0} -> Lemma
   (((a * ((r * r) % n)) / r) % n == (a * r) % n)
-let lemma_mod_div_simplify a r n = admit()
+let lemma_mod_div_simplify a r n =
+    let res = ((a * ((r * r) % n)) / r) % n in
+    lemma_mod_mult_div (r * r) a r n;
+    assert (res == ((a * r * r) / r) % n);
+    paren_mul_left a r r;
+    assert (res == (((a * r) * r) / r) % n);
+    multiple_division_lemma (a * r) r
 
 val lemma_mont_reduction:
 	res:nat -> r:nat{r > 0} -> c:nat -> n:nat{n > 0} -> m:nat -> Lemma
-	(requires (res = (c + m * n) / r))
+	(requires (res = (c + m * n) / r /\ res < n + n))
 	(ensures (res % n == (c / r) % n))
-let lemma_mont_reduction res r c n m = admit()
+let lemma_mont_reduction res r c n m =
+    let res = (c + m * n) / r in
+    assert (res % n == ((c + m * n) / r) % n);
+    lemma_mod_mult_div_1 (c + m * n) r n;
+    assert (res % n == (((c + m * n) % n) / r) % n);
+    lemma_mod_plus c m n;
+    //assert ((c + m * n) % n == c % n);
+    //assert (res % n == ((c % n) / r) % n);
+    lemma_mod_mult_div_1 c r n
+    //assert (res % n == (c / r) % n)
+
+val lemma_mont_reduction_1:
+	res:nat -> r:nat{r > 0} -> c:nat -> n:nat{n > 0} -> m:nat -> Lemma
+	(requires (res = (c + m * n) / r /\ res < n))
+	(ensures (res == (c / r) % n))
+let lemma_mont_reduction_1 res r c n m =
+    lemma_mont_reduction res r c n m;
+    assert (res % n == (c / r) % n);
+    small_modulo_lemma_1 res n;
+	assert (res % n == res);
+    assert (res == (c / r) % n)
+
+(* LEMMAS for modular exponentiation *)
+#reset-options "--z3rlimit 30 --max_fuel 0"
+val lemma_r_n:
+    modBits:nat -> r:nat -> n:nat -> Lemma
+    (requires (r == pow2 (modBits + 2) /\ n < pow2 modBits))
+    (ensures (4 * n < r))
+let lemma_r_n modBits r n =
+    pow2_plus 2 modBits;
+	assert_norm (pow2 2 = 4);
+	pow2_lt_compat (2 + modBits) modBits;
+	assert (pow2 modBits < 4 * pow2 modBits);
+	assert (4 * n < r)
+
+#reset-options "--z3rlimit 150 --max_fuel 0"
+
+val lemma_mod_exp:
+	n:nat{n > 1} -> a:nat -> a2:nat ->
+	b:nat -> b2:nat -> acc:nat -> r:nat{r > 0} -> res:nat -> Lemma
+	(requires (a2 % n == (a * a / r) % n /\ b2 == b / 2 /\ 
+              res % n == ((pow a2 b2) * acc / pow r b2) % n))
+	(ensures (res % n == ((pow a (2 * b2)) * acc / pow r (2 * b2)) % n))
+let lemma_mod_exp n a a2 b b2 acc r res =
+    assert (res % n == ((pow a2 b2) * acc / pow r b2) % n);
+    lemma_mod_mult_div (pow a2 b2) acc (pow r b2) n;
+    //assert (res % n == (((pow a2 b2) % n) * acc / pow r b2) % n);
+    lemma_pow_mod a2 b2 n;
+    //assert ((pow a2 b2) % n == (pow (a2 % n) b2) % n);
+    //assert ((pow a2 b2) % n == (pow ((a * a / r) % n) b2) % n);
+    lemma_pow_mod (a * a / r) b2 n;
+    //assert ((pow a2 b2) % n == (pow (a * a / r) b2) % n);
+    lemma_pow_div (a * a) b2 r;
+    //assert ((pow a2 b2) % n == ((pow (a * a) b2) / pow r b2) % n);
+    lemma_pow_a2_b a b2;
+    //assert ((pow a2 b2) % n == (pow a (2 * b2) / pow r b2) % n);
+    //assert (res % n == (((pow a (2 * b2) / pow r b2) % n) * acc / pow r b2) % n);
+    lemma_mod_mult_div (pow a (2 * b2) / pow r b2) acc (pow r b2) n;
+    //assert (res % n == (((pow a (2 * b2) / pow r b2) * acc) / pow r b2) % n);
+    lemma_mod_mult_div_1 ((pow a (2 * b2) / pow r b2) * acc) (pow r b2) n;
+    //assert (res % n == ((((pow a (2 * b2) / pow r b2) * acc) % n) / pow r b2) % n);
+    lemma_mult_div_mod acc (pow a (2 * b2)) (pow r b2) n;
+    //assert (res % n == ((((acc * pow a (2 * b2)) / pow r b2) % n) / pow r b2) % n);
+    lemma_mod_mult_div_1 ((acc * pow a (2 * b2)) / pow r b2) (pow r b2) n;
+    //assert (res % n == (((acc * pow a (2 * b2)) / pow r b2) / pow r b2) % n);
+    division_multiplication_lemma (acc * pow a (2 * b2)) (pow r b2) (pow r b2);
+    //assert (res % n == ((acc * pow a (2 * b2)) / (pow r b2 * pow r b2)) % n);
+    lemma_pow r b2 b2
+    //assert (pow r b2 * pow r b2 == pow r (2 * b2))
+
+#reset-options "--z3rlimit 150 --max_fuel 0"
+
+val lemma_mod_exp_1:
+	n:nat{n > 1} -> a:nat -> a2:nat ->
+	b:nat -> b2:nat -> acc:nat -> acc':nat -> r:nat{r > 0} -> res:nat -> Lemma
+	(requires (a2 % n == (a * a / r) % n /\ b2 == b / 2 /\ 
+               res % n == ((pow a2 b2) * acc' / pow r b2) % n /\
+               acc' % n == (a * acc / r) % n))
+	(ensures (res % n == ((pow a (2 * b2 + 1)) * acc / pow r (2 * b2 + 1)) % n))
+let lemma_mod_exp_1 n a a2 b b2 acc acc' r res =
+    lemma_mod_exp n a a2 b b2 acc' r res;
+    //assert (res % n == ((pow a (2 * b2)) * acc' / pow r (2 * b2)) % n);
+    lemma_mod_mult_div acc' (pow a (2 * b2)) (pow r (2 * b2)) n;
+    //assert (res % n == ((pow a (2 * b2)) * ((a * acc / r) % n) / pow r (2 * b2)) % n);
+    lemma_mod_mult_div (a * acc / r) (pow a (2 * b2)) (pow r (2 * b2)) n;
+    //assert (res % n == (((pow a (2 * b2)) * (a * acc / r)) / pow r (2 * b2)) % n);
+    lemma_mod_mult_div_1 ((pow a (2 * b2)) * (a * acc / r)) (pow r (2 * b2)) n;
+    //assert (res % n == ((((pow a (2 * b2)) * (a * acc / r)) % n) / pow r (2 * b2)) % n);
+    lemma_mult_div_mod (pow a (2 * b2)) (a * acc) r n;
+    //assert (res % n == ((((pow a (2 * b2)) * (a * acc) / r) % n) / pow r (2 * b2)) % n);
+    lemma_mod_mult_div_1 ((pow a (2 * b2)) * (a * acc) / r) ( pow r (2 * b2)) n;
+    //assert (res % n == (((pow a (2 * b2)) * (a * acc) / r) / pow r (2 * b2)) % n);
+    division_multiplication_lemma ((pow a (2 * b2)) * (a * acc)) r (pow r (2 * b2));
+    //assert (res % n == (((pow a (2 * b2)) * (a * acc)) / (r * pow r (2 * b2))) % n);
+    paren_mul_right (pow a (2 * b2)) a acc;
+    assert_norm (pow a 1 = a);
+    assert_norm (pow r 1 = r);
+    lemma_pow a 1 (2 * b2);
+    lemma_pow r 1 (2 * b2);
+    assert (a * pow a (2 * b2) = pow a (2 * b2 + 1));
+    assert (r * pow r (2 * b2) = pow r (2 * b2 + 1));
+    assert (res % n == ((pow a (2 * b2 + 1)) * acc / pow r (2 * b2 + 1)) % n)
+
+#reset-options "--z3rlimit 300 --max_fuel 0"
+
+val lemma_mod_exp_2:
+	n:nat{n > 1} -> a:nat -> a_r:nat ->
+	b:nat -> acc_r:nat -> r:nat{r > 0} -> res_r:nat -> Lemma
+	(requires (a_r % n == (a * r) % n /\ acc_r % n == r % n /\
+               res_r % n == ((pow a_r b) * acc_r / pow r b) % n))
+	(ensures (res_r % n == ((pow a b) * r) % n))
+let lemma_mod_exp_2 n a a_r b acc_r r res_r =
+    assert (res_r % n == ((pow a_r b) * acc_r / pow r b) % n);
+    lemma_mod_mult_div (pow a_r b) acc_r (pow r b) n;
+    //assert (res_r % n == (((pow a_r b) % n) * acc_r / pow r b) % n);
+    lemma_pow_mod a_r b n;
+    //assert ((pow a_r b) % n == (pow (a_r % n) b) % n);
+    //assert ((pow a_r b) % n == (pow ((a * r) % n) b) % n);
+    lemma_pow_mod (a * r) b n;  
+    //assert ((pow a_r b) % n == (pow (a * r) b) % n);
+    lemma_pow_mul a r b;
+    //assert ((pow a_r b) % n == ((pow a b) * (pow r b)) % n);
+    assert (res_r % n == ((((pow a b) * (pow r b)) % n) * acc_r / pow r b) % n);
+    lemma_mod_mult_div ((pow a b) * (pow r b)) acc_r (pow r b) n;
+    assert (res_r % n == (((pow a b) * (pow r b) * acc_r) / pow r b) % n);
+    assert (res_r % n == (((pow a b) * acc_r * pow r b) / pow r b) % n);
+    multiple_division_lemma ((pow a b) * acc_r) (pow r b);
+    //assert (res_r % n == ((pow a b) * acc_r) % n);
+    lemma_mod_mul_distr_l acc_r (pow a b) n;
+    //assert (res_r % n == ((acc_r % n) * pow a b) % n);
+    //assert (res_r % n == ((r % n) * pow a b) % n);
+    lemma_mod_mul_distr_l r (pow a b) n;
+    assert (res_r % n == (r * pow a b) % n)
